More

CpcMini/SmtModel.lean
@@ -731,9 +731,7 @@ def __smtx_model_eval_fun (M : SmtModel) (fid : native_Nat) (U : SmtType) (i : S
     fallback
   else
     match __smtx_model_fun_lookup M fid with
-    | some f =>
-      let v := f i
-      (native_ite (native_Teq (__smtx_typeof_value v) U) v fallback)
+    | some f => f i
     | none => fallback
 
 def __smtx_model_eval_apply (M : SmtModel) : SmtValue -> SmtValue -> SmtValue
@@ -1101,10 +1099,18 @@ def type_inhabited (T : SmtType) : Prop :=
 def __smtx_value_canonical (v : SmtValue) : Prop :=
   __smtx_value_canonical_bool v = true
 
+def native_fun_typed (M : SmtModel) : Prop :=
+  ∀ fid A B i,
+    __smtx_type_wf (SmtType.FunType A B) = true ->
+    __smtx_typeof_value i = A ->
+    __smtx_typeof_value (__smtx_model_eval_fun M fid B i) = B ∧
+      __smtx_value_canonical (__smtx_model_eval_fun M fid B i)
+
 def model_total_typed (M : SmtModel) : Prop :=
   (∀ s T, __smtx_type_wf T = true -> __smtx_typeof_value (__smtx_model_lookup M s T) = T) ∧
   (∀ s T, __smtx_type_wf T = true -> __smtx_value_canonical (__smtx_model_lookup M s T)) ∧
-  (∀ s T, __smtx_type_wf T = false -> __smtx_model_lookup M s T = SmtValue.NotValue)
+  (∀ s T, __smtx_type_wf T = false -> __smtx_model_lookup M s T = SmtValue.NotValue) ∧
+  native_fun_typed M
 
 /-
 SMT interpretation is satisfiability, i.e. the existence of a model
